chapter05-dsm/solutions/elide-types.dfy
@@ -1,0 +1,9 @@
+// Elided from student dir; simply directly-included into solutions
+// and given models
+module CommitTypes {
+  // How a particular participant feels.
+  datatype Vote = Yes | No
+  // What decision has been reached by the protocol.
+  datatype Decision = Commit | Abort
+}
+
