chapter05-dsm/solutions/model_for_ex03.dfy
@@ -1,7 +1,8 @@
+//#desc Given model for exercise03
 // This file is an "official solution" to exercises 01 & 02, to ensure you're
 // not doing battle with mistakes in your own protocol definition.  The proof
 // is challenging enough for an exercise without fighting protocol bugs.
-//#inline "exercise02.dfy"
+//#inline "exercise02_solution.dfy"
 //#start-elide
-include "exercise02.dfy"
+include "exercise02_solution.dfy"
 //#end-elide
