chapter06-refine/solutions/impl_model_for_ex04.dfy
@@ -1,0 +1,11 @@
+//#desc Implementation state machine for refinement proof in exercise04.
+
+// This file is an instructor-supplied solution to the 2PC implementation in
+// chapter 5, so you're not doing battle with an implementation that's
+// impossible to prove. In fact, you can reuse parts of the instructor-supplied
+// proof from here as well.
+// 
+//#inlineinclude "../../chapter05-dsm/solutions/exercise03_solution.dfy"
+//#start-elide
+include "../../chapter05-dsm/solutions/exercise03_solution.dfy"
+//#end-elide
