chapter06-refine/solutions/spec_model_for_ex04.dfy
@@ -1,0 +1,9 @@
+//#desc Specification state machine for refinement proof in exercise04.
+
+// This file is an instructor-provided solution to the Atomic Commit spec in
+// exercise02, so you're not doing battle with a spec that's impossible to
+// satisfy -- or getting away with refining to a spec that's trivial.
+//#inlineinclude "exercise02_solution.dfy"
+//#start-elide
+include "exercise02_solution.dfy"
+//#end-elide
